code/experimental/gcm/Hacl.Standalone.GMAC.fst
@@ -1,5 +1,6 @@
 module Hacl.Standalone.GMAC
 
+module U8   = FStar.UInt8
 module U32  = FStar.UInt32
 module H8   = Hacl.UInt8
 module H128 = Hacl.UInt128
@@ -10,78 +11,121 @@ open Spec.GF128
 open Hacl.Impl.GF128
 
 open FStar.Mul
+open FStar.HyperStack
 open FStar.Seq
 open FStar.Buffer
 open FStar.Endianness
-open Hacl.Cast
+open Hacl.Endianness
 
-(* GMAC state *)
-noeq type gmac_state = {r_acc:buffer H128.t; s_pmsg_len:buffer H8.t}
-
-let live_st h (st:gmac_state) : Type0 =
-  live h st.r_acc /\ live h st.s_pmsg_len /\ disjoint st.r_acc st.s_pmsg_len
-
-let valid_st h (st:gmac_state) : Type0 =
-  live_st h st /\ length st.r_acc = 2 /\ length st.s_pmsg_len = 33 /\
-  H8.v (get h st.s_pmsg_len 32) < 16
-
-
-(* Get information from state *)
 #set-options "--z3rlimit 20 --initial_fuel 0 --max_fuel 0 --initial_ifuel 0 --max_ifuel 0"
 
-private val h8_to_u32: x:H8.t -> GTot (u:U32.t{H8.v x = U32.v u})
-let h8_to_u32 x = 
-  let cast (x:nat{x < pow2 32 - 1}) : GTot (UInt.uint_t 32) = x in
-  assert(H8.v x < pow2 32 - 1);
-  U32.uint_to_t (cast (H8.v x))
+(* GMAC state *)
+noeq type gmac_state = {ram:buffer H128.t; len:buffer U32.t}
 
+private let decode_pmsg (pmsg:H128.t) (len:U32.t{U32.v len <= 16}) : GTot word =
+  slice (big_bytes 16ul (H128.v pmsg)) 0 (U32.v len)
+
+let live_st h (st:gmac_state) : Type0 =
+  live h st.ram /\ live h st.len /\ disjoint st.ram st.len
+
+let valid_pmsg (pmsg:H128.t) (len:U32.t) : Type0 =
+  U32.v len < 16 /\ pad (decode_pmsg pmsg len) = big_bytes 16ul (H128.v pmsg)
+
+let valid_st h (st:gmac_state) : Type0 =
+  live_st h st /\ length st.ram = 3 /\ length st.len = 1 /\
+  valid_pmsg (get h st.ram 2) (get h st.len 0)
+  
+
+(* Get information from state *)
+  
 private let get_r h (st:gmac_state{valid_st h st}) : GTot elem =
-  sel_elem h (sub st.r_acc 0ul 1ul)
-private let get_s h (st:gmac_state{valid_st h st}) : GTot tag =
-  as_seq h (sub st.s_pmsg_len 0ul 16ul)
+  sel_elem h (sub st.ram 0ul 1ul)
 private let get_acc h (st:gmac_state{valid_st h st}) : GTot elem =
-  sel_elem h (sub st.r_acc 1ul 1ul)
-private let get_pmsg h (st:gmac_state{valid_st h st}) : GTot (pmsg:bytes{Seq.length pmsg < 16}) =
-  as_seq h (sub st.s_pmsg_len 16ul (h8_to_u32 (get h st.s_pmsg_len 32)))
+  sel_elem h (sub st.ram 1ul 1ul)
+private let get_pmsg h (st:gmac_state{valid_st h st}) :
+  GTot (pmsg:bytes{Seq.length pmsg = U32.v (get h st.len 0)}) =
+  decode_pmsg (get h st.ram 2) (get h st.len 0)
 
 private val as_pure_st: h:HyperStack.mem -> st:gmac_state{valid_st h st} -> GTot (pst:gmac_state_)
-let as_pure_st h st = MkState (get_r h st) (get_s h st) (get_acc h st) (get_pmsg h st)
+let as_pure_st h st = MkState (get_r h st) (get_acc h st) (get_pmsg h st)
 
 
 #reset-options "--z3rlimit 50 --initial_fuel 0 --max_fuel 0 --initial_ifuel 0 --max_ifuel 0"
 
-val gmac_init: st:gmac_state -> r:wordB_16{disjoint st.r_acc r /\ disjoint st.s_pmsg_len r} ->
-  s:tagB{disjoint st.r_acc s /\ disjoint st.s_pmsg_len s /\ disjoint r s} -> Stack unit
-  (requires (fun h -> valid_st h st /\ live h r /\ live h s))
-  (ensures (fun h0 _ h1 -> valid_st h0 st /\ live h0 r /\ live h0 s /\
-    valid_st h1 st /\ live h1 r /\ live h1 s /\ modifies_2 st.r_acc st.s_pmsg_len h0 h1 /\
-    as_pure_st h1 st == gmac_init_spec (as_seq h0 r) (as_seq h0 s)))
-let gmac_init st r s =
+(* Useful lemmas *)
+
+private let valid_pmsg_ (pmsg:H128.t) (len:U32.t) : Type0 =
+  U32.v len < 16 /\ H128.v pmsg % (pow2 (8 * (16 - U32.v len))) = 0
+
+private val zero_div_mod: n:pos -> Lemma (0 / n = 0 /\ 0 % n = 0)
+let zero_div_mod n = ()
+
+private val lemma_is_valid_pmsg_: pmsg:H128.t -> len:U32.t{valid_pmsg_ pmsg len} -> i:nat{i < 16 - U32.v len} ->
+  Lemma (requires True)
+  (ensures (Seq.index (slice (big_bytes 16ul (H128.v pmsg)) (U32.v len) 16) i = 0uy))
+  [SMTPat (Seq.index (slice (big_bytes 16ul (H128.v pmsg)) (U32.v len) 16) i)]
+let lemma_is_valid_pmsg_ pmsg len i =
+  lemma_index_big_bytes 16ul (H128.v pmsg) (U32.v len + i);
+  Math.Lemmas.pow2_modulo_division_lemma_1 (H128.v pmsg) (8 * (16 - U32.v len - i - 1)) (8 * (16 - U32.v len - i));
+  Math.Lemmas.pow2_modulo_modulo_lemma_1 (H128.v pmsg) (8 * (16 - U32.v len - i)) (8 * (16 - U32.v len));
+  zero_div_mod (pow2 (8 * (16 - U32.v len - i)));
+  zero_div_mod (pow2 (8 * (16 - U32.v len - i - 1)))
+  
+private val lemma_is_valid_pmsg: pmsg:H128.t -> len:U32.t -> Lemma
+  (requires (valid_pmsg_ pmsg len))
+  (ensures (valid_pmsg pmsg len))
+  [SMTPat (valid_pmsg pmsg len)]
+let lemma_is_valid_pmsg pmsg len =
+  lemma_eq_intro (Seq.create (16 - U32.v len) 0uy) (slice (big_bytes 16ul (H128.v pmsg)) (U32.v len) 16);
+  lemma_eq_intro (pad (decode_pmsg pmsg len)) (big_bytes 16ul (H128.v pmsg))
+  
+
+(* Main functions *)
+
+#reset-options "--z3rlimit 80 --initial_fuel 0 --max_fuel 0 --initial_ifuel 0 --max_ifuel 0"
+
+val gmac_alloc: unit -> StackInline gmac_state
+  (requires (fun _ -> True))
+  (ensures (fun h0 st h1 -> ~(contains h0 st.ram) /\
+    frameOf st.ram == h0.tip /\ frameOf st.len == h0.tip /\
+    modifies_0 h0 h1 /\ valid_st h1 st))
+let gmac_alloc () =
+  let ram = create zero_128 3ul in
+  let len = create 0ul 1ul in
+  {ram = ram; len = len}
+
+val gmac_init: st:gmac_state -> r:keyB{disjoint st.ram r /\ disjoint st.len r} -> Stack unit
+  (requires (fun h -> valid_st h st /\ live h r))
+  (ensures (fun h0 _ h1 -> valid_st h0 st /\ live h0 r /\ valid_st h1 st /\ live h1 r /\
+    modifies_2 st.ram st.len h0 h1 /\
+    as_pure_st h1 st = gmac_init_spec (sel_word h0 r)))
+let gmac_init st r =
   let h0 = ST.get() in
-  let st_r = sub st.r_acc 0ul 1ul in
-  let rv = load128_be r in
-  st_r.(0ul) <- rv;
-  let st_s = sub st.s_pmsg_len 0ul 16ul in
-  blit s 0ul st_s 0ul 16ul;
-  let st_acc = sub st.r_acc 1ul 1ul in
-  st_acc.(0ul) <- zero_128;
-  let st_len = sub st.s_pmsg_len 32ul 1ul in
-  st_len.(0ul) <- uint8_to_sint8 0uy;
+  let rv = encodeB r in
+  st.ram.(0ul) <- rv;
+  st.ram.(1ul) <- zero_128;
+  st.ram.(2ul) <- zero_128;
+  st.len.(0ul) <- 0ul;
   let h1 = ST.get() in
-  (* valid_st h1 st *)
-  lemma_sub_spec st.s_pmsg_len 32ul 1ul h1;
-  Seq.lemma_index_slice (as_seq h1 st.s_pmsg_len) 32 33 0;
-  (* get_r h1 st = encode (as_seq h0 r) *)
-  Seq.lemma_eq_intro (get_r h1 st) (encode (as_seq h0 r));
-  (* get_s h1 st = as_seq h0 s *)
-  Seq.lemma_eq_intro (Seq.slice (get_s h1 st) 0 16) (get_s h1 st);
-  Seq.lemma_eq_intro (Seq.slice (as_seq h0 s) 0 16) (as_seq h0 s);
-  Seq.lemma_eq_intro (get_s h1 st) (as_seq h0 s);
-  (* get_acc h1 st = zero *)
+  zero_div_mod (pow2 (8 * 16));
+  Seq.lemma_eq_intro (get_r h1 st) (encode (sel_word h0 r));
   fzero_lemma zero_128;
   Seq.lemma_eq_intro (get_acc h1 st) zero;
-  lemma_sub_spec st.s_pmsg_len 16ul (h8_to_u32 (get h1 st.s_pmsg_len 32)) h1;
   Seq.lemma_eq_intro (get_pmsg h1 st) (Seq.createEmpty)
+
+private val update_pmsg: pmsg:H128.t -> len_1:U32.t{valid_pmsg_ pmsg len_1} ->
+  nmsg:wordB -> len_2:U32.t{length nmsg = U32.v len_2 /\ U32.(v (len_1 +^ len_2)) <= 16} -> StackInline H128.t
+  (requires (fun h -> live h nmsg))
+  (ensures (fun h0 r h1 -> h0 == h1 /\ live h0 nmsg /\ 
+    decode_pmsg r U32.(len_1 +^ len_2) = decode_pmsg pmsg len_1 @| sel_word h0 nmsg))
+let update_pmsg pmsg len_1 nmsg len_2 = admit()
+
+val gmac_update: st:gmac_state -> msg:buffer H8.t{disjoint st.ram msg /\ disjoint st.len msg} -> Stack unit
+  (requires (fun h -> valid_st h st /\ live h msg))
+  (ensures (fun h0 _ h1 -> valid_st h0 st /\ live h0 msg /\ valid_st h1 st /\ live h1 msg /\
+    modifies_2 st.ram st.len h0 h1 /\
+    as_pure_st h1 st = gmac_update_spec (as_pure_st h0 st) (sel_word h0 msg)))
+let gmac_update st msg = admit()
 
 
 (*
